src/PurePrimops.ec
@@ -1,19 +1,21 @@
 pragma Goals:printall.
 
 require import Array.
-require import IntDiv.
-require import Logic.
 require import Memory.
+require import Ring.
+        import Ring.IntID.
 require export UInt256.
 require import Utils.
 
 theory PurePrimops.
 
+import MemoryMap.
+
 (* definitions ========== *)
 
 (* uninterpreted functions *)
 op calldata : uint256 array.
-op keccak256_f : uint256 array -> uint256.
+op keccak256_f : uint8 array -> uint256.
 
 
 op iszero(v : uint256) : uint256 = if (v = W256.zero) then W256.one else  W256.zero
@@ -25,21 +27,8 @@ axiomatized by gt_uint256E.
 op slt_uint256 (x y : uint256) = if uint256_as_signed x < uint256_as_signed y then W256.one else W256.zero
 axiomatized by slt_uint256E.
 
-(* arithmetic definition *)
-(* could also be done bitwise *)
-op mload_bit (memory: mem) (idx: uint256) (i: int): bool =
-  memory.[idx + W256.of_int (i %/ 8)].[i %% 8].
-op mload (memory: mem) (idx: uint256): uint256 =
-  W256.init (mload_bit memory idx).
-op mstore_bit (memory: mem) (idx: uint256) (i: int) (bit: bool): mem =
-  let byte_index = idx + W256.of_int (i %/ 8) in
-  let byte = memory.[byte_index] in
-  memory.[byte_index <- (byte.[i%%8 <- bit])].
-op mstore_uint8 (memory: mem) (idx: uint256) (val: uint8): mem =
-  
-    
-
-op mstore (memory: mem) (idx val: uint256): mem.
+abbrev mload = load.
+abbrev mstore = store.
 
 op mulmod(a b n : uint256) : uint256 =
   let a_int = W256.to_uint a in
@@ -64,6 +53,9 @@ axiomatized by shlE.
 op shr(a : uint256, b : uint256) : uint256 = a `>>>` (W256.to_uint b)
 axiomatized by shrE.
 
+op modexp(base: uint256, exponent: uint256, mod: uint256) = W256.of_int (((W256.to_uint base) ^ (W256.to_uint exponent)) %% (W256.to_uint mod))
+axiomatized by modexpE.
+
 op STRING : uint256 = W256.zero.
 
 
@@ -82,140 +74,5 @@ lemma iszero_nonzeroE (val: uint256) : val <> W256.zero => iszero val = W256.zer
       rewrite /iszero.
       smt ().
   qed.
-
-(* mstore *)
-op words_overlap (address1 address2: uint256) =
-  (exists (offset: int), 0 <= offset /\ offset < 32 /\ address1 + W256.of_int offset = address2) \/
-  (exists (offset: int), 0 <= offset /\ offset < 32 /\ address2 + W256.of_int offset = address1)
-  axiomatized by words_overlapE.
-
-lemma subK (a b c: uint256): a - b <> a - c => b <> c.
-    proof.
-      progress.
-      (* smt (@W256). *)
-      smt iterate.
-  qed.
-
-lemma sub_self (a: uint256): a - a = W256.zero.
-    proof.
-      smt (@W256).
-  qed.
-
-lemma sub_add (a b c: uint256): a - (b + c) = a - b - c.
-    proof.
-      admit.
-      (* smt timeout=1000. *)
-  qed.
-
-lemma mod_of_lt (a b: int): 0 < a => 0 < b => a < b => a %% b = a.
-    proof.
-      smt ().
-  qed.
-
-lemma get_right (a b c: int): a <= b < c => b < c.
-    proof.
-      smt().
-    qed.
-
-lemma add_neq_of_lt (idx idx2: uint256) (offset: int):
-    W256.of_int 31 < idx2 - idx =>  0 <= offset /\ offset < 32 => (idx + W256.of_int offset) <> idx2.
-    proof.
-      progress.
-      rewrite W256.ultE W256.of_uintK in H.
-      apply (subK idx2).
-      rewrite sub_self.
-      rewrite sub_add.
-      rewrite /W256.ulift2.
-      have Lifted: W256.of_int (W256.to_uint (idx2 - idx) - offset) <> W256.of_int 0.
-      pose diff := to_uint (idx2 - idx).
-      have diff_gt:  31 < diff.
-      rewrite /diff.
-      rewrite (mod_of_lt 31 W256.modulus) in H; trivial.
-      have diff_lt: diff < W256.modulus.
-      rewrite /diff.
-      exact (get_right 0 (to_uint (idx2 - idx)) W256.modulus (W256.to_uint_cmp (idx2 - idx))).
-      smt (@W256).
-      smt (@W256).
-  qed.
-
-lemma no_overlap (idx idx2: uint256):
-    W256.of_int 31 < idx - idx2 => W256.of_int 31 < idx2 - idx => !words_overlap idx idx2.
-    proof.
-      progress.
-      smt (add_neq_of_lt).
-  qed.
-
-op uint256_frame (memory_pre memory_post: mem) (idx: uint256) = forall (idx2: uint256), W256.of_int 31 < idx2 - idx => memory_post.[idx2] = memory_pre.[idx2].
-
-axiom mload_mstore_same (memory: mem) (idx val: uint256):
-  mload (mstore memory idx val) idx = val.
-
-axiom mstore_frame (memory: mem) (idx val: uint256):
-  uint256_frame memory (mstore memory idx val) idx.
-
-axiom mstore_preserves_wellformed (memory: mem) (idx val: uint256):
-  mem_wellformed memory => mem_wellformed (mstore memory idx val).
-
-axiom mstore_mloaded_val (memory: mem) (idx: uint256):
-  mstore memory idx (mload memory idx) = memory.
-
-axiom mstore_of_load_and_frame (memory_pre memory_post: mem) (idx val: uint256):
-  mem_wellformed memory_pre =>
-  mem_wellformed memory_post =>
-  mload memory_post idx = val =>
-  uint256_frame memory_pre memory_post idx =>
-  memory_post = mstore memory_pre idx val.
-
-lemma apply_mstore_mload_diff (memory: mem) (idx idx2 val: uint256):
-    W256.of_int 31 < idx2 - idx => W256.of_int 31 < idx - idx2 =>  mload (mstore memory idx val) idx2 = mload memory idx2.
-proof.
-  progress.
-  rewrite /mload.
-  pose memory_post := mstore memory idx val.
-  have h_full: mload memory_post idx = val /\ uint256_frame memory memory_post idx. by smt.
-  have h_frame: uint256_frame memory memory_post idx. smt.
-  rewrite /uint256_frame in h_frame.
-  have h31: forall (offset: int), 0 <= offset => offset < 32 => memory_post.[idx2 + W256.of_int offset] = memory.[idx2 + W256.of_int offset].
-  progress.
-  apply h_frame.
-  rewrite /W256.\ult.
-  rewrite W256.of_uintK.
-  rewrite mod_of_lt; trivial.
-  by smt timeout=100.
-  have h0: memory_post.[idx2] = memory.[idx2] by smt.
-  (rewrite (h31 31); first trivial); first trivial.
-  (rewrite (h31 30); first trivial); first trivial.
-  (rewrite (h31 29); first trivial); first trivial.
-  (rewrite (h31 28); first trivial); first trivial.
-  (rewrite (h31 27); first trivial); first trivial.
-  (rewrite (h31 26); first trivial); first trivial.
-  (rewrite (h31 25); first trivial); first trivial.
-  (rewrite (h31 24); first trivial); first trivial.
-  (rewrite (h31 23); first trivial); first trivial.
-  (rewrite (h31 22); first trivial); first trivial.
-  (rewrite (h31 21); first trivial); first trivial.
-  (rewrite (h31 20); first trivial); first trivial.
-  (rewrite (h31 19); first trivial); first trivial.
-  (rewrite (h31 18); first trivial); first trivial.
-  (rewrite (h31 17); first trivial); first trivial.
-  (rewrite (h31 16); first trivial); first trivial.
-  (rewrite (h31 15); first trivial); first trivial.
-  (rewrite (h31 14); first trivial); first trivial.
-  (rewrite (h31 13); first trivial); first trivial.
-  (rewrite (h31 12); first trivial); first trivial.
-  (rewrite (h31 11); first trivial); first trivial.
-  (rewrite (h31 10); first trivial); first trivial.
-  (rewrite (h31 9); first trivial); first trivial.
-  (rewrite (h31 8); first trivial); first trivial.
-  (rewrite (h31 7); first trivial); first trivial.
-  (rewrite (h31 6); first trivial); first trivial.
-  (rewrite (h31 5); first trivial); first trivial.
-  (rewrite (h31 4); first trivial); first trivial.
-  (rewrite (h31 3); first trivial); first trivial.
-  (rewrite (h31 2); first trivial); first trivial.
-  (rewrite (h31 1); first trivial); first trivial.
-    rewrite h0.
-    reflexivity.
-qed.
 
 end PurePrimops.
