src/YulPrimops.ec
@@ -1,171 +1,40 @@
 pragma Goals:printall.
 
-require import AllCore Int IntDiv.
+require import AllCore.
 require import Array.
+require import Int.
+require import IntDiv.
 require import Logic.
 require import PurePrimops.
 require import Utils.
-require export UInt256 Memory EllipticCurve.
+require export EllipticCurve.
+require export Memory.
+require export UInt256.
+
+import MemoryMap.
 
 module Primops = {
   var memory : mem
-  var ret_data : uint256 array
+  var ret_data : mem
   var reverted : bool
 
   proc mload(idx : uint256) : uint256 = {
-    (* _1 is the most significant byte *)
-    (* TODO replace definition with a direct call to op mload *)
-    var _r1, _r2, _r3, _r4, _r5, _r6, _r7, _r8, _r9, _r10, _r11, _r12, _r13, _r14, _r15, _r16, _r17, _r18, _r19, _r20, _r21, _r22, _r23, _r24, _r25, _r26, _r27, _r28, _r29, _r30, _r31, _r32;
-
-
-    _r1 <- memory.[idx] `<<<` 248;
-    _r2 <- memory.[idx+ W256.of_int 1] `<<<` 240;
-    _r3 <- memory.[idx+ W256.of_int 2] `<<<` 232;
-    _r4 <- memory.[idx+ W256.of_int 3] `<<<` 224;
-    _r5 <- memory.[idx+ W256.of_int 4] `<<<` 216;
-    _r6 <- memory.[idx+ W256.of_int 5] `<<<` 208;
-    _r7 <- memory.[idx+ W256.of_int 6] `<<<` 200;
-    _r8 <- memory.[idx+ W256.of_int 7] `<<<` 192;
-    _r9 <- memory.[idx+ W256.of_int 8] `<<<` 184;
-    _r10 <- memory.[idx+ W256.of_int 9] `<<<` 176;
-    _r11 <- memory.[idx+ W256.of_int 10] `<<<` 168;
-    _r12 <- memory.[idx+ W256.of_int 11] `<<<` 160;
-    _r13 <- memory.[idx+ W256.of_int 12] `<<<` 152;
-    _r14 <- memory.[idx+ W256.of_int 13] `<<<` 144;
-    _r15 <- memory.[idx+ W256.of_int 14] `<<<` 136;
-    _r16 <- memory.[idx+ W256.of_int 15] `<<<` 128;
-    _r17 <- memory.[idx+ W256.of_int 16] `<<<` 120;
-    _r18 <- memory.[idx+ W256.of_int 17] `<<<` 112;
-    _r19 <- memory.[idx+ W256.of_int 18] `<<<` 104;
-    _r20 <- memory.[idx+ W256.of_int 19] `<<<` 96;
-    _r21 <- memory.[idx+ W256.of_int 20] `<<<` 88;
-    _r22 <- memory.[idx+ W256.of_int 21] `<<<` 80;
-    _r23 <- memory.[idx+ W256.of_int 22] `<<<` 72;
-    _r24 <- memory.[idx+ W256.of_int 23] `<<<` 64;
-    _r25 <- memory.[idx+ W256.of_int 24] `<<<` 56;
-    _r26 <- memory.[idx+ W256.of_int 25] `<<<` 48;
-    _r27 <- memory.[idx+ W256.of_int 26] `<<<` 40;
-    _r28 <- memory.[idx+ W256.of_int 27] `<<<` 32;
-    _r29 <- memory.[idx+ W256.of_int 28] `<<<` 24;
-    _r30 <- memory.[idx+ W256.of_int 29] `<<<` 16;
-    _r31 <- memory.[idx+ W256.of_int 30] `<<<` 8;
-    _r32 <- memory.[idx+ W256.of_int 31];
-
-    return (
-      _r32 +
-      _r31 +
-      _r30 +
-      _r29 +
-      _r28 +
-      _r27 +
-      _r26 +
-      _r25 +
-      _r24 +
-      _r23 +
-      _r22 +
-      _r21 +
-      _r20 +
-      _r19 +
-      _r18 +
-      _r17 +
-      _r16 +
-      _r15 +
-      _r14 +
-      _r13 +
-      _r12 +
-      _r11 +
-      _r10 +
-      _r9 +
-      _r8 +
-      _r7 +
-      _r6 +
-      _r5 +
-      _r4 +
-      _r3 +
-      _r2 +
-      _r1
-    );
+    return (PurePrimops.mload memory idx);
   }
 
   proc mstore(idx : uint256, val : uint256): unit = {
-    var  _w248,  _w240,  _w232,  _w224,  _w216,  _w208,  _w200,  _w192,  _w184,  _w176,  _w168,  _w160,  _w152,  _w144,  _w136,  _w128,  _w120,  _w112,  _w104,  _w96,  _w88,  _w80,  _w72,  _w64,  _w56,  _w48,  _w40,  _w32,  _w24,  _w16,  _w8,  _w0;
-     _w248 <- splitMask (W256.masklsb 248) val;
-     _w240 <- splitMask (W256.masklsb 240) ( _w248.`1);
-     _w232 <- splitMask (W256.masklsb 232) ( _w240.`1);
-     _w224 <- splitMask (W256.masklsb 224) ( _w232.`1);
-     _w216 <- splitMask (W256.masklsb 216) ( _w224.`1);
-     _w208 <- splitMask (W256.masklsb 208) ( _w216.`1);
-     _w200 <- splitMask (W256.masklsb 200) ( _w208.`1);
-     _w192 <- splitMask (W256.masklsb 192) ( _w200.`1);
-     _w184 <- splitMask (W256.masklsb 184) ( _w192.`1);
-     _w176 <- splitMask (W256.masklsb 176) ( _w184.`1);
-     _w168 <- splitMask (W256.masklsb 168) ( _w176.`1);
-     _w160 <- splitMask (W256.masklsb 160) ( _w168.`1);
-     _w152 <- splitMask (W256.masklsb 152) ( _w160.`1);
-     _w144 <- splitMask (W256.masklsb 144) ( _w152.`1);
-     _w136 <- splitMask (W256.masklsb 136) ( _w144.`1);
-     _w128 <- splitMask (W256.masklsb 128) ( _w136.`1);
-     _w120 <- splitMask (W256.masklsb 120) ( _w128.`1);
-     _w112 <- splitMask (W256.masklsb 112) ( _w120.`1);
-     _w104 <- splitMask (W256.masklsb 104) ( _w112.`1);
-     _w96 <- splitMask (W256.masklsb 96) ( _w104.`1);
-     _w88 <- splitMask (W256.masklsb 88) ( _w96.`1);
-     _w80 <- splitMask (W256.masklsb 80) ( _w88.`1);
-     _w72 <- splitMask (W256.masklsb 72) ( _w80.`1);
-     _w64 <- splitMask (W256.masklsb 64) ( _w72.`1);
-     _w56 <- splitMask (W256.masklsb 56) ( _w64.`1);
-     _w48 <- splitMask (W256.masklsb 48) ( _w56.`1);
-     _w40 <- splitMask (W256.masklsb 40) ( _w48.`1);
-     _w32 <- splitMask (W256.masklsb 32) ( _w40.`1);
-     _w24 <- splitMask (W256.masklsb 24) ( _w32.`1);
-     _w16 <- splitMask (W256.masklsb 16) ( _w24.`1);
-     _w8 <- splitMask (W256.masklsb 8) ( _w16.`1);
-     _w0 <- splitMask (W256.masklsb 0) ( _w8.`1);
-
-    memory <- memory.[idx<- _w248.`2 `>>>` 248];
-    memory <- memory.[(idx+W256.of_int 1)<-_w240.`2 `>>>` 240];
-    memory <- memory.[(idx+W256.of_int 2)<-_w232.`2 `>>>` 232];
-    memory <- memory.[(idx+W256.of_int 3)<-_w224.`2 `>>>` 224];
-    memory <- memory.[(idx+W256.of_int 4)<-_w216.`2 `>>>` 216];
-    memory <- memory.[(idx+W256.of_int 5)<-_w208.`2 `>>>` 208];
-    memory <- memory.[(idx+W256.of_int 6)<-_w200.`2 `>>>` 200];
-    memory <- memory.[(idx+W256.of_int 7)<-_w192.`2 `>>>` 192];
-    memory <- memory.[(idx+W256.of_int 8)<-_w184.`2 `>>>` 184];
-    memory <- memory.[(idx+W256.of_int 9)<-_w176.`2 `>>>` 176];
-    memory <- memory.[(idx+W256.of_int 10)<-_w168.`2 `>>>` 168];
-    memory <- memory.[(idx+W256.of_int 11)<-_w160.`2 `>>>` 160];
-    memory <- memory.[(idx+W256.of_int 12)<-_w152.`2 `>>>` 152];
-    memory <- memory.[(idx+W256.of_int 13)<-_w144.`2 `>>>` 144];
-    memory <- memory.[(idx+W256.of_int 14)<-_w136.`2 `>>>` 136];
-    memory <- memory.[(idx+W256.of_int 15)<-_w128.`2 `>>>` 128];
-    memory <- memory.[(idx+W256.of_int 16)<-_w120.`2 `>>>` 120];
-    memory <- memory.[(idx+W256.of_int 17)<-_w112.`2 `>>>` 112];
-    memory <- memory.[(idx+W256.of_int 18)<-_w104.`2 `>>>` 104];
-    memory <- memory.[(idx+W256.of_int 19)<-_w96.`2 `>>>` 96];
-    memory <- memory.[(idx+W256.of_int 20)<-_w88.`2 `>>>` 88];
-    memory <- memory.[(idx+W256.of_int 21)<-_w80.`2 `>>>` 80];
-    memory <- memory.[(idx+W256.of_int 22)<-_w72.`2 `>>>` 72];
-    memory <- memory.[(idx+W256.of_int 23)<-_w64.`2 `>>>` 64];
-    memory <- memory.[(idx+W256.of_int 24)<-_w56.`2 `>>>` 56];
-    memory <- memory.[(idx+W256.of_int 25)<-_w48.`2 `>>>` 48];
-    memory <- memory.[(idx+W256.of_int 26)<-_w40.`2 `>>>` 40];
-    memory <- memory.[(idx+W256.of_int 27)<-_w32.`2 `>>>` 32];
-    memory <- memory.[(idx+W256.of_int 28)<-_w24.`2 `>>>` 24];
-    memory <- memory.[(idx+W256.of_int 29)<-_w16.`2 `>>>` 16];
-    memory <- memory.[(idx+W256.of_int 30)<-_w8.`2 `>>>` 8];
-    memory <- memory.[(idx+W256.of_int 31)<-_w0.`2 `>>>` 0];
+    memory <- PurePrimops.mstore memory idx val;
   }
 
   proc mstore8(idx : uint256, val : uint256) : unit = {
-    memory <- memory.[idx<-(val `&` W256.masklsb 8)];
+    memory <- memory.[idx<-W8.of_int (W256.to_uint val)];
   }
 
   proc evm_return(retOff : uint256, retSize : uint256) : unit = {
       var i : uint256;
       i <- W256.zero;
-      ret_data <- Array.mkarray (List.nseq (W256.to_uint retSize) W256.zero);
       while (i < retSize) {
-      ret_data.[W256.to_uint i] <- memory.[retOff + i];
+      ret_data <- ret_data.[i <- memory.[retOff + i]];
       i <- i + W256.one;
       }
       return ();
@@ -178,15 +47,8 @@ module Primops = {
 
   proc keccak256(off : uint256, size : uint256) : uint256 = {
       (* TODO: relate to keccak_f *)
-      var input : uint256 array;
-      var i : uint256;
-      i <- W256.zero;
-      input <- Array.mkarray (List.nseq (W256.to_uint size) W256.zero);
-      while (i < size) {
-      input.[W256.to_uint i] <- memory.[off + i];
-      i <- i + W256.one;
-      }
-    
+      var input : uint8 array;
+      input <- Array.offun (fun (i: int) => memory.[off + (W256.of_int i)]) (W256.to_uint size);
       return PurePrimops.keccak256_f input;
   }
 
@@ -301,9 +163,7 @@ phoare [ Primops.mload :
       proc.
       wp.
       skip.
-      progress.
-      rewrite /mload.
-      reflexivity.
+      by progress.
   qed.
 
 lemma mload_spec (memory: mem) (idx: uint256):
@@ -318,17 +178,14 @@ hoare [ Primops.mload :
       proc.
       wp.
       skip.
-      progress.
-      rewrite /mload.
-      reflexivity.
+      by progress.
   qed.
     
 lemma mstore_pspec:
     forall (memory: mem) (idx': uint256) (val': uint256),
 phoare [ Primops.mstore :
     arg = (idx', val') /\
-    Primops.memory = memory /\
-    mem_wellformed memory ==>
+    Primops.memory = memory  ==>
       Primops.memory = PurePrimops.mstore memory idx' val'
     ] = 1%r.
     proof.
@@ -336,198 +193,14 @@ phoare [ Primops.mstore :
       proc.
       wp.
       skip.
-    move => &hr h_args.
-      have h_idx: idx{hr} = idx'.
-      smt.
-      have h_val: val{hr} = val'.
-      admit. (* TODO add sufficient weakening lemmas to utils *)
-      have h_mem: Primops.memory{hr} = memory.
-      smt.
-    move => x248 x240 x232 x224 x216 x208 x200 x192 x184 x176 x168 x160 x152 x144 x136 x128 x120 x112 x104 x96 x88 x80 x72 x64 x56 x48 x40 x32 x24 x16 x8.
-      apply PurePrimops.mstore_of_load_and_frame.
-      smt ().
-      do 32! (rewrite write_byte_maintains_wellformed; first admit). (* mem wellformedness *)
-      smt ().
-      rewrite h_mem.
-      rewrite /mload.
-      rewrite h_idx.
-      rewrite {1} Map.get_set_sameE.
-      rewrite {1} get_set_offsets_neq; first trivial.
-      rewrite {1} Map.get_set_sameE.
-      rewrite masklsb_zero.
-      rewrite splitMask_zero.
-      rewrite shr_zero.
-      rewrite /x8.
-      rewrite splitMask2_shr_shl; first trivial.
-      rewrite splitMask_add.
-      do 2! (rewrite {1} get_set_offsets_neq; first trivial).
-      rewrite {1} Map.get_set_sameE.
-      rewrite /x16.
-      rewrite splitMask2_shr_shl; first trivial.
-      rewrite splitMask_add.
-      do 3! (rewrite {1} get_set_offsets_neq; first trivial).
-      rewrite {1} Map.get_set_sameE.
-      rewrite /x24.
-      rewrite splitMask2_shr_shl; first trivial.
-      rewrite splitMask_add.    
-      do 4! (rewrite {1} get_set_offsets_neq; first trivial).
-      rewrite {1} Map.get_set_sameE.
-      rewrite /x32.
-      rewrite splitMask2_shr_shl; first trivial.
-      rewrite splitMask_add.    
-      do 5! (rewrite {1} get_set_offsets_neq; first trivial).
-      rewrite {1} Map.get_set_sameE.
-      rewrite /x40.
-      rewrite splitMask2_shr_shl; first trivial.
-      rewrite splitMask_add.    
-      do 6! (rewrite {1} get_set_offsets_neq; first trivial).
-      rewrite {1} Map.get_set_sameE.
-      rewrite /x48.
-      rewrite splitMask2_shr_shl; first trivial.
-      rewrite splitMask_add.
-      do 7! (rewrite {1} get_set_offsets_neq; first trivial).
-      rewrite {1} Map.get_set_sameE.
-      rewrite /x56.
-      rewrite splitMask2_shr_shl; first trivial.
-      rewrite splitMask_add.
-      do 8! (rewrite {1} get_set_offsets_neq; first trivial).
-      rewrite {1} Map.get_set_sameE.
-      rewrite /x64.
-      rewrite splitMask2_shr_shl; first trivial.
-      rewrite splitMask_add.
-      do 9! (rewrite {1} get_set_offsets_neq; first trivial).
-      rewrite {1} Map.get_set_sameE.
-      rewrite /x72.
-      rewrite splitMask2_shr_shl; first trivial.
-      rewrite splitMask_add.
-      do 10! (rewrite {1} get_set_offsets_neq; first trivial).
-      rewrite {1} Map.get_set_sameE.
-      rewrite /x80.
-      rewrite splitMask2_shr_shl; first trivial.
-      rewrite splitMask_add.
-      do 11! (rewrite {1} get_set_offsets_neq; first trivial).
-      rewrite {1} Map.get_set_sameE.
-      rewrite /x88.
-      rewrite splitMask2_shr_shl; first trivial.
-      rewrite splitMask_add.
-      do 12! (rewrite {1} get_set_offsets_neq; first trivial).
-      rewrite {1} Map.get_set_sameE.
-      rewrite /x96.
-      rewrite splitMask2_shr_shl; first trivial.
-      rewrite splitMask_add.
-      do 13! (rewrite {1} get_set_offsets_neq; first trivial).
-      rewrite {1} Map.get_set_sameE.
-      rewrite /x104.
-      rewrite splitMask2_shr_shl; first trivial.
-      rewrite splitMask_add.
-      do 14! (rewrite {1} get_set_offsets_neq; first trivial).
-      rewrite {1} Map.get_set_sameE.
-      rewrite /x112.
-      rewrite splitMask2_shr_shl; first trivial.
-      rewrite splitMask_add.
-      do 15! (rewrite {1} get_set_offsets_neq; first trivial).
-      rewrite {1} Map.get_set_sameE.
-      rewrite /x120.
-      rewrite splitMask2_shr_shl; first trivial.
-      rewrite splitMask_add.
-      do 16! (rewrite {1} get_set_offsets_neq; first trivial).
-      rewrite {1} Map.get_set_sameE.
-      rewrite /x128.
-      rewrite splitMask2_shr_shl; first trivial.
-      rewrite splitMask_add.
-      do 17! (rewrite {1} get_set_offsets_neq; first trivial).
-      rewrite {1} Map.get_set_sameE.
-      rewrite /x136.
-      rewrite splitMask2_shr_shl; first trivial.
-      rewrite splitMask_add.
-      do 18! (rewrite {1} get_set_offsets_neq; first trivial).
-      rewrite {1} Map.get_set_sameE.
-      rewrite /x144.
-      rewrite splitMask2_shr_shl; first trivial.
-      rewrite splitMask_add.
-      do 19! (rewrite {1} get_set_offsets_neq; first trivial).
-      rewrite {1} Map.get_set_sameE.
-      rewrite /x152.
-      rewrite splitMask2_shr_shl; first trivial.
-      rewrite splitMask_add.
-      do 20! (rewrite {1} get_set_offsets_neq; first trivial).
-      rewrite {1} Map.get_set_sameE.
-      rewrite /x160.
-      rewrite splitMask2_shr_shl; first trivial.
-      rewrite splitMask_add.
-      do 21! (rewrite {1} get_set_offsets_neq; first trivial).
-      rewrite {1} Map.get_set_sameE.
-      rewrite /x168.
-      rewrite splitMask2_shr_shl; first trivial.
-      rewrite splitMask_add.
-      do 22! (rewrite {1} get_set_offsets_neq; first trivial).
-      rewrite {1} Map.get_set_sameE.
-      rewrite /x176.
-      rewrite splitMask2_shr_shl; first trivial.
-      rewrite splitMask_add.
-      do 23! (rewrite {1} get_set_offsets_neq; first trivial).
-      rewrite {1} Map.get_set_sameE.
-      rewrite /x184.
-      rewrite splitMask2_shr_shl; first trivial.
-      rewrite splitMask_add.
-      do 24! (rewrite {1} get_set_offsets_neq; first trivial).
-      rewrite {1} Map.get_set_sameE.
-      rewrite /x192.
-      rewrite splitMask2_shr_shl; first trivial.
-      rewrite splitMask_add.
-      do 25! (rewrite {1} get_set_offsets_neq; first trivial).
-      rewrite {1} Map.get_set_sameE.
-      rewrite /x200.
-      rewrite splitMask2_shr_shl; first trivial.
-      rewrite splitMask_add.
-      do 26! (rewrite {1} get_set_offsets_neq; first trivial).
-      rewrite {1} Map.get_set_sameE.
-      rewrite /x208.
-      rewrite splitMask2_shr_shl; first trivial.
-      rewrite splitMask_add.
-      do 27! (rewrite {1} get_set_offsets_neq; first trivial).
-      rewrite {1} Map.get_set_sameE.
-      rewrite /x216.
-      rewrite splitMask2_shr_shl; first trivial.
-      rewrite splitMask_add.
-      do 28! (rewrite {1} get_set_offsets_neq; first trivial).
-      rewrite {1} Map.get_set_sameE.
-      rewrite /x224.
-      rewrite splitMask2_shr_shl; first trivial.
-      rewrite splitMask_add.
-      do 29! (rewrite {1} get_set_offsets_neq; first trivial).
-      rewrite {1} Map.get_set_sameE.
-      rewrite /x232.
-      rewrite splitMask2_shr_shl; first trivial.
-      rewrite splitMask_add.
-      do 30! (rewrite {1} get_set_offsets_neq; first trivial).
-      rewrite {1} Map.get_set_sameE.
-      rewrite /x240.
-      rewrite splitMask2_shr_shl; first trivial.
-      rewrite splitMask_add.
-      do 31! (rewrite {1} get_set_offset; first trivial).
-      rewrite {1} Map.get_set_sameE.
-      rewrite /x248.
-      rewrite splitMask2_shr_shl; first trivial.
-      rewrite splitMask_add.
-      exact h_val.
-      rewrite /uint256_frame.
-    move => idx2 h_idx2.
-      rewrite h_idx.
-      do 31! (rewrite {1} Map.get_set_neqE; first by smt (PurePrimops.add_neq_of_lt)).
-      rewrite Map.get_set_neqE.
-      apply neq_of_lt.
-      exact h_idx2.
-      rewrite h_mem.
-      reflexivity.
-  qed.
+      by progress.
+    qed.
 
 lemma mstore_spec:
     forall (memory: mem) (idx': uint256) (val': uint256),
 hoare [ Primops.mstore :
     arg = (idx', val') /\
-    Primops.memory = memory /\
-    mem_wellformed memory ==>
+    Primops.memory = memory ==>
       Primops.memory = PurePrimops.mstore memory idx' val'
     ].
     proof.
@@ -535,190 +208,166 @@ hoare [ Primops.mstore :
       proc.
       wp.
       skip.
-    move => &hr h_args.
-      have h_idx: idx{hr} = idx'.
-      smt.
-      have h_val: val{hr} = val'.
-      admit. (* TODO add sufficient weakening lemmas to utils *)
-      have h_mem: Primops.memory{hr} = memory.
-      smt.
-    move => x248 x240 x232 x224 x216 x208 x200 x192 x184 x176 x168 x160 x152 x144 x136 x128 x120 x112 x104 x96 x88 x80 x72 x64 x56 x48 x40 x32 x24 x16 x8.
-      apply PurePrimops.mstore_of_load_and_frame.
-      smt ().
-      do 32! (rewrite write_byte_maintains_wellformed; first admit). (* mem wellformedness *)
-      smt ().
-      rewrite h_mem.
-      rewrite /mload.
-      rewrite h_idx.
-      rewrite {1} Map.get_set_sameE.
-      rewrite {1} get_set_offsets_neq; first trivial.
-      rewrite {1} Map.get_set_sameE.
-      rewrite masklsb_zero.
-      rewrite splitMask_zero.
-      rewrite shr_zero.
-      rewrite /x8.
-      rewrite splitMask2_shr_shl; first trivial.
-      rewrite splitMask_add.
-      do 2! (rewrite {1} get_set_offsets_neq; first trivial).
-      rewrite {1} Map.get_set_sameE.
-      rewrite /x16.
-      rewrite splitMask2_shr_shl; first trivial.
-      rewrite splitMask_add.
-      do 3! (rewrite {1} get_set_offsets_neq; first trivial).
-      rewrite {1} Map.get_set_sameE.
-      rewrite /x24.
-      rewrite splitMask2_shr_shl; first trivial.
-      rewrite splitMask_add.    
-      do 4! (rewrite {1} get_set_offsets_neq; first trivial).
-      rewrite {1} Map.get_set_sameE.
-      rewrite /x32.
-      rewrite splitMask2_shr_shl; first trivial.
-      rewrite splitMask_add.    
-      do 5! (rewrite {1} get_set_offsets_neq; first trivial).
-      rewrite {1} Map.get_set_sameE.
-      rewrite /x40.
-      rewrite splitMask2_shr_shl; first trivial.
-      rewrite splitMask_add.    
-      do 6! (rewrite {1} get_set_offsets_neq; first trivial).
-      rewrite {1} Map.get_set_sameE.
-      rewrite /x48.
-      rewrite splitMask2_shr_shl; first trivial.
-      rewrite splitMask_add.
-      do 7! (rewrite {1} get_set_offsets_neq; first trivial).
-      rewrite {1} Map.get_set_sameE.
-      rewrite /x56.
-      rewrite splitMask2_shr_shl; first trivial.
-      rewrite splitMask_add.
-      do 8! (rewrite {1} get_set_offsets_neq; first trivial).
-      rewrite {1} Map.get_set_sameE.
-      rewrite /x64.
-      rewrite splitMask2_shr_shl; first trivial.
-      rewrite splitMask_add.
-      do 9! (rewrite {1} get_set_offsets_neq; first trivial).
-      rewrite {1} Map.get_set_sameE.
-      rewrite /x72.
-      rewrite splitMask2_shr_shl; first trivial.
-      rewrite splitMask_add.
-      do 10! (rewrite {1} get_set_offsets_neq; first trivial).
-      rewrite {1} Map.get_set_sameE.
-      rewrite /x80.
-      rewrite splitMask2_shr_shl; first trivial.
-      rewrite splitMask_add.
-      do 11! (rewrite {1} get_set_offsets_neq; first trivial).
-      rewrite {1} Map.get_set_sameE.
-      rewrite /x88.
-      rewrite splitMask2_shr_shl; first trivial.
-      rewrite splitMask_add.
-      do 12! (rewrite {1} get_set_offsets_neq; first trivial).
-      rewrite {1} Map.get_set_sameE.
-      rewrite /x96.
-      rewrite splitMask2_shr_shl; first trivial.
-      rewrite splitMask_add.
-      do 13! (rewrite {1} get_set_offsets_neq; first trivial).
-      rewrite {1} Map.get_set_sameE.
-      rewrite /x104.
-      rewrite splitMask2_shr_shl; first trivial.
-      rewrite splitMask_add.
-      do 14! (rewrite {1} get_set_offsets_neq; first trivial).
-      rewrite {1} Map.get_set_sameE.
-      rewrite /x112.
-      rewrite splitMask2_shr_shl; first trivial.
-      rewrite splitMask_add.
-      do 15! (rewrite {1} get_set_offsets_neq; first trivial).
-      rewrite {1} Map.get_set_sameE.
-      rewrite /x120.
-      rewrite splitMask2_shr_shl; first trivial.
-      rewrite splitMask_add.
-      do 16! (rewrite {1} get_set_offsets_neq; first trivial).
-      rewrite {1} Map.get_set_sameE.
-      rewrite /x128.
-      rewrite splitMask2_shr_shl; first trivial.
-      rewrite splitMask_add.
-      do 17! (rewrite {1} get_set_offsets_neq; first trivial).
-      rewrite {1} Map.get_set_sameE.
-      rewrite /x136.
-      rewrite splitMask2_shr_shl; first trivial.
-      rewrite splitMask_add.
-      do 18! (rewrite {1} get_set_offsets_neq; first trivial).
-      rewrite {1} Map.get_set_sameE.
-      rewrite /x144.
-      rewrite splitMask2_shr_shl; first trivial.
-      rewrite splitMask_add.
-      do 19! (rewrite {1} get_set_offsets_neq; first trivial).
-      rewrite {1} Map.get_set_sameE.
-      rewrite /x152.
-      rewrite splitMask2_shr_shl; first trivial.
-      rewrite splitMask_add.
-      do 20! (rewrite {1} get_set_offsets_neq; first trivial).
-      rewrite {1} Map.get_set_sameE.
-      rewrite /x160.
-      rewrite splitMask2_shr_shl; first trivial.
-      rewrite splitMask_add.
-      do 21! (rewrite {1} get_set_offsets_neq; first trivial).
-      rewrite {1} Map.get_set_sameE.
-      rewrite /x168.
-      rewrite splitMask2_shr_shl; first trivial.
-      rewrite splitMask_add.
-      do 22! (rewrite {1} get_set_offsets_neq; first trivial).
-      rewrite {1} Map.get_set_sameE.
-      rewrite /x176.
-      rewrite splitMask2_shr_shl; first trivial.
-      rewrite splitMask_add.
-      do 23! (rewrite {1} get_set_offsets_neq; first trivial).
-      rewrite {1} Map.get_set_sameE.
-      rewrite /x184.
-      rewrite splitMask2_shr_shl; first trivial.
-      rewrite splitMask_add.
-      do 24! (rewrite {1} get_set_offsets_neq; first trivial).
-      rewrite {1} Map.get_set_sameE.
-      rewrite /x192.
-      rewrite splitMask2_shr_shl; first trivial.
-      rewrite splitMask_add.
-      do 25! (rewrite {1} get_set_offsets_neq; first trivial).
-      rewrite {1} Map.get_set_sameE.
-      rewrite /x200.
-      rewrite splitMask2_shr_shl; first trivial.
-      rewrite splitMask_add.
-      do 26! (rewrite {1} get_set_offsets_neq; first trivial).
-      rewrite {1} Map.get_set_sameE.
-      rewrite /x208.
-      rewrite splitMask2_shr_shl; first trivial.
-      rewrite splitMask_add.
-      do 27! (rewrite {1} get_set_offsets_neq; first trivial).
-      rewrite {1} Map.get_set_sameE.
-      rewrite /x216.
-      rewrite splitMask2_shr_shl; first trivial.
-      rewrite splitMask_add.
-      do 28! (rewrite {1} get_set_offsets_neq; first trivial).
-      rewrite {1} Map.get_set_sameE.
-      rewrite /x224.
-      rewrite splitMask2_shr_shl; first trivial.
-      rewrite splitMask_add.
-      do 29! (rewrite {1} get_set_offsets_neq; first trivial).
-      rewrite {1} Map.get_set_sameE.
-      rewrite /x232.
-      rewrite splitMask2_shr_shl; first trivial.
-      rewrite splitMask_add.
-      do 30! (rewrite {1} get_set_offsets_neq; first trivial).
-      rewrite {1} Map.get_set_sameE.
-      rewrite /x240.
-      rewrite splitMask2_shr_shl; first trivial.
-      rewrite splitMask_add.
-      do 31! (rewrite {1} get_set_offset; first trivial).
-      rewrite {1} Map.get_set_sameE.
-      rewrite /x248.
-      rewrite splitMask2_shr_shl; first trivial.
-      rewrite splitMask_add.
-      exact h_val.
-      rewrite /uint256_frame.
-    move => idx2 h_idx2.
-      rewrite h_idx.
-      do 31! (rewrite {1} Map.get_set_neqE; first by smt (PurePrimops.add_neq_of_lt)).
-      rewrite Map.get_set_neqE.
-      apply neq_of_lt.
-      exact h_idx2.
-      rewrite h_mem.
+      by progress.
+  qed.
+
+lemma keccak256_pspec (off size: uint256):
+    phoare [ Primops.keccak256 :
+      arg = (off, size) ==>
+      res = PurePrimops.keccak256_f(Array.offun (fun (i: int) => Primops.memory.[off + (W256.of_int i)]) (W256.to_uint size))
+    ] = 1%r.
+    proof.
+      proc.
+      wp.
+      skip.
+      by progress.
+  qed.
+
+lemma calldataload_pspec (idx: uint256):
+    phoare [Primops.calldataload:
+      arg = idx ==>
+      res = PurePrimops.calldata.[W256.to_uint idx]
+    ] = 1%r.
+    proof.
+      proc.
+      wp.
+      skip.
+      by progress.
+  qed.
+
+lemma staticcall_modexp_spec (memory: mem) (a b c gas argOff retOff: uint256):
+    hoare [ Primops.staticcall:
+      arg = (gas, W256.of_int 5, argOff, W256.of_int 192, retOff, W256.of_int 32) /\
+      Primops.memory = memory /\
+      PurePrimops.mload memory argOff = W256.of_int 32 /\
+      PurePrimops.mload memory (argOff + (W256.of_int 32)) = W256.of_int 32 /\
+      PurePrimops.mload memory (argOff + (W256.of_int 64)) = W256.of_int 32 /\
+      PurePrimops.mload memory (argOff + (W256.of_int 96)) = a /\
+      PurePrimops.mload memory (argOff + (W256.of_int 128)) = b /\
+      PurePrimops.mload memory (argOff + (W256.of_int 160)) = c ==>
+    Primops.memory = PurePrimops.mstore memory retOff (PurePrimops.modexp a b c) /\
+      res = W256.one
+    ].
+    proof.
+      proc.
+      rcondt 1. skip. by progress.
+      seq 3 : (#pre /\ bsize = W256.of_int 32 /\ esize = W256.of_int 32 /\ msize = W256.of_int 32).
+      inline Primops.mload. wp. skip. by progress.
+      rcondt 1. skip. by progress.
+      seq 3 : (#pre /\ base = a /\ exp = b /\ mod = c).
+      inline Primops.mload. wp. skip. by progress.
+      wp.
+      call (ConcretePrimops.mstore_spec memory retOff (PurePrimops.modexp a b c)).
+      skip.
+      progress.
+      rewrite PurePrimops.modexpE.
       reflexivity.
+  qed.
+
+lemma staticcall_modexp_pspec (memory: mem) (a b c gas argOff retOff: uint256):
+    phoare [ Primops.staticcall:
+      arg = (gas, W256.of_int 5, argOff, W256.of_int 192, retOff, W256.of_int 32) /\
+      Primops.memory = memory /\
+      PurePrimops.mload memory argOff = W256.of_int 32 /\
+      PurePrimops.mload memory (argOff + (W256.of_int 32)) = W256.of_int 32 /\
+      PurePrimops.mload memory (argOff + (W256.of_int 64)) = W256.of_int 32 /\
+      PurePrimops.mload memory (argOff + (W256.of_int 96)) = a /\
+      PurePrimops.mload memory (argOff + (W256.of_int 128)) = b /\
+      PurePrimops.mload memory (argOff + (W256.of_int 160)) = c ==>
+    Primops.memory = PurePrimops.mstore memory retOff (PurePrimops.modexp a b c) /\
+      res = W256.one
+    ] = 1%r.
+    proof.
+      proc.
+      rcondt 1. skip. by progress.
+      rcondt 4.
+      inline Primops.mload. wp. skip. by progress.
+      wp.
+      call (ConcretePrimops.mstore_pspec memory retOff (PurePrimops.modexp a b c)).
+      inline Primops.mload. wp. skip.
+      progress.
+      rewrite PurePrimops.modexpE.
+      reflexivity.
+  qed.
+
+lemma is_none_iff_not_is_some (a: 'a option): is_none a <=> !is_some a.
+    proof.
+      case (a = None). smt (). smt ().
     qed.
+
+pred point_wellformed (pnt: uint256*uint256) =
+    pnt.`1 = pnt.`1 %% W256.of_int p /\
+    pnt.`2 = pnt.`2 %% W256.of_int p.
+pred point_oncurve (pnt: uint256*uint256) =
+    on_curve ((ZModField.inzmod(to_sint pnt.`1)), (ZModField.inzmod(to_sint pnt.`2))).
+pred staticcall_ec_add_should_succeed (p1 p2: uint256 * uint256) =
+    point_wellformed p1 /\
+    point_wellformed p2 /\
+    point_oncurve p1 /\
+    point_oncurve p2 /\
+    is_some (ecAdd_precompile (ZModField.inzmod(to_sint p1.`1)) (ZModField.inzmod(to_sint p1.`2)) (ZModField.inzmod(to_sint p2.`1)) (ZModField.inzmod(to_sint p2.`2))).
+
+op ecAdd_precompile_unsafe_cast (p1 p2: uint256 * uint256): (uint256*uint256) =
+  let x1 = ZModField.inzmod(to_sint p1.`1) in
+  let y1 = ZModField.inzmod(to_sint p1.`2) in
+  let x2 = ZModField.inzmod(to_sint p2.`1) in
+  let y2 = ZModField.inzmod(to_sint p2.`2) in
+  let ret = ecAdd_precompile x1 y1 x2 y2 in
+  let ret_unwrapped = odflt (ZModField.zero, ZModField.zero) ret in
+  let x_ret = W256.of_int (ZModField.asint ret_unwrapped.`1) in
+  let y_ret = W256.of_int (ZModField.asint ret_unwrapped.`2) in
+  (x_ret,y_ret).
+
+lemma staticcall_ec_add_pspec (memory: mem) (p1 p2: uint256 * uint256) (argOff retOff: uint256):
+    phoare [ Primops.staticcall :
+      arg = (gas, W256.of_int 6, argOff, W256.of_int 128, retOff, W256.of_int 64) /\
+      Primops.memory = memory /\
+      p1.`1 = PurePrimops.mload memory argOff /\
+      p1.`2 = PurePrimops.mload memory (argOff + W256.of_int 32) /\
+      p2.`1 = PurePrimops.mload memory (argOff + W256.of_int 64) /\
+      p2.`2 = PurePrimops.mload memory (argOff + W256.of_int 96)
+      ==>
+      ((staticcall_ec_add_should_succeed p1 p2) => (
+        res = W256.one /\
+        Primops.memory = PurePrimops.mstore
+          (PurePrimops.mstore
+            memory
+            retOff
+            (ecAdd_precompile_unsafe_cast p1 p2).`1
+          )
+          (retOff + W256.of_int 32)
+          (ecAdd_precompile_unsafe_cast p1 p2).`2
+      )) /\
+      ((!staticcall_ec_add_should_succeed p1 p2) => res = W256.zero /\ Primops.memory = memory)
+    ] = 1%r.
+    proof.
+      proc.
+      inline *.
+      rcondf 1. skip. progress. by smt(@W256).
+      rcondt 1. skip. by progress.
+    case (staticcall_ec_add_should_succeed p1 p2).
+      rcondf 13. wp. skip. progress. by smt().
+      rcondf 13. wp. skip. progress. by smt ().
+      rcondf 14. wp. skip. progress. by smt (is_none_iff_not_is_some).
+      wp. skip. progress.
+      rewrite /ecAdd_precompile_unsafe_cast.
+      simplify.
+      smt ().
+      smt (). smt ().
+    case (!point_wellformed p1 \/ !point_wellformed p2).
+      rcondt 13. wp. skip. progress. by smt ().
+      wp. skip. by progress.
+      rcondf 13. wp. skip. progress. by smt ().
+    case (!point_oncurve p1 \/ !point_oncurve p2).
+      rcondt 13. wp. skip. progress. by smt ().
+      wp. skip. by progress.
+      rcondf 13. wp. skip. progress. by smt ().
+      rcondt 14. wp. skip. progress. by smt ().
+      wp. skip. by progress.
+    qed.
+      
+
+
+    
 
 end ConcretePrimops.
