src/specs/Wheels.ec
@@ -1,3 +1,0 @@
-theory Primops.
-op reverted: bool.
-end Primops.
